extraction/src/JuraParser.mly
@@ -27,8 +27,9 @@
 
 %token IF GUARD ELSE
 %token RETURN THROW
-%token LET
+%token LET AS
 %token NEW THIS
+%token SWITCH TYPESWITCH CASE DEFAULT
 
 %token OR AND NOT
 %token FLATTEN
@@ -207,6 +208,8 @@ expr:
     { JuraCompiler.jthis }
 | LET v = safeident EQUAL e1 = expr SEMI e2 = expr
     { JuraCompiler.jlet v e1 e2 }
+| SWITCH e0 = expr LCURLY csd = cases RCURLY
+    { JuraCompiler.jswitch e0 (fst csd) (snd csd) }
 (* Functions *)
 | NOT e = expr
     { JuraCompiler.junaryop JuraCompiler.Ops.Unary.opneg e }
@@ -269,6 +272,19 @@ exprlist:
 | e = expr COMMA el = exprlist
     { e :: el }
 
+(* cases *)
+cases:
+| DEFAULT COLON e = expr
+    { ([],e) }
+| CASE d = data COLON e = expr cs = cases
+    { (((None,JuraCompiler.jcasevalue d),e)::(fst cs), snd cs) }
+| CASE LET v = safeident EQUAL d = data COLON e = expr cs = cases
+    { (((Some v,JuraCompiler.jcasevalue d),e)::(fst cs), snd cs) }
+| CASE AS brand = STRING COLON e = expr tcs = cases
+    { (((None,JuraCompiler.jcasetype (Util.char_list_of_string brand)),e)::(fst tcs), snd tcs) }
+| CASE LET v = safeident AS brand = STRING COLON e = expr tcs = cases
+    { (((Some v,JuraCompiler.jcasetype (Util.char_list_of_string brand)),e)::(fst tcs), snd tcs) }
+
 (* New struct *)
 reclist:
 | 
@@ -312,6 +328,14 @@ qname_prefix:
       | (Some prefix, last) -> Util.char_list_of_string (prefix ^ "." ^ last)
       end }
 
+(* data *)
+data:
+| s = STRING
+    { JuraCompiler.Data.dstring (Util.char_list_of_string s) }
+| i = INT
+    { JuraCompiler.Data.dnat i }
+| f = FLOAT
+    { JuraCompiler.Enhanced.Data.dfloat f }
 (* Safe identifier *)
 safeident:
 | i = safeident_base
@@ -332,7 +356,12 @@ safeident_base:
 | THROW { "throw" }
 | THROWS { "throws" }
 | LET { "let" }
+| AS { "as" }
 | NEW { "new" }
+| SWITCH { "switch" }
+| TYPESWITCH { "typeswitch" }
+| CASE { "case" }
+| DEFAULT { "default" }
 | THIS { "this" }
 | OR { "or" }
 | AND { "and" }
