BUILD.md
@@ -26,7 +26,7 @@ necessary libraries as follow:
 ```
 $ opam repo add coq-released https://coq.inria.fr/opam/released
 $ opam install ocamlbuild menhir camlp5 base64 js_of_ocaml js_of_ocaml-ppx
-$ opam install coq.8.7.1 coq-qcert.1.0.4
+$ opam install coq.8.7.2 coq-qcert.1.0.5
 ```
 
 ### Build the Jura Compiler
