doc/Notes.md
@@ -1,0 +1,21 @@
+Compilation for switch expressions:
+
+```
+[[ switch e0 {
+     case let v1 as type1: e1
+     case let v2 as type2: e2
+     default: edefault
+   } ]]
+==
+let v0 := [[ e0 ]] in
+  match cast v0 as type1
+  | left as v1 -> [[ e1 ]]
+  | right as _v1 ->
+    match cast v0 as type2
+    | left as v2 -> [[ e2 ]]
+    | right as _v2 -> [[ edefault ]]
+```
+
+with `v0` fresh in `[[e1]]`, `[[e2]]` and `[[edefault]]` `_v1` fresh
+in `[[e2]]` and `[[edefault]]` and `_v2` fresh in `[[edefault]]`.
+
